resolve comment
reflect comment

fix typo

src/Vellvm/opsem.v
@@ -555,13 +555,13 @@ Proof.
   destruct (zeq z 0); simpl in DECISION; rewrite DECISION; auto.
 Qed.
 
-Inductive decide_nonzero_with_undef (TD:TargetData) (gv gvs1 gvs2 gvundef gvresult:GenericValue) (t:typ) (decision:option bool): Prop :=
-| decide_nonzero_def
+Inductive calc_select (TD:TargetData) (t:typ) (gv gvs1 gvs2 gvresult:GenericValue) : Prop :=
+| select_cond_def
     z
     (INT: GV2int TD Size.One gv = Some z)
-    (DECISION: decision = Some (negb (zeq z 0)))
     (RESULT: gvresult = if (negb (zeq z 0)) then gvs1 else gvs2)
-| decide_nonzero_undef
+| select_cond_undef
+    gvundef
     (NOINT: GV2int TD Size.One gv = None)
     (UNDEF: gundef TD t = Some gvundef)
     (RESULT: gvresult = gvundef)
@@ -844,12 +844,12 @@ Inductive sInsn : Config -> State -> State -> trace -> Prop :=
     (mkState (mkEC F B cs tmn (updateAddAL _ lc id gvs3) als) (ECS) Mem)
     E0
 
-| sSelect : forall S TD Ps F B lc gl fs id v0 t v1 v2 c ECS cs tmn Mem als decision
-                    gvs1 gvs2 gvundef gvresult,
+| sSelect : forall S TD Ps F B lc gl fs id v0 t v1 v2 c ECS cs tmn Mem als
+                    gvs1 gvs2 gvresult,
   getOperandValue TD v0 lc gl = Some c ->
   getOperandValue TD v1 lc gl = Some gvs1 ->
   getOperandValue TD v2 lc gl = Some gvs2 ->
-  decide_nonzero_with_undef TD c gvs1 gvs2 gvundef gvresult t decision ->
+  calc_select TD t c gvs1 gvs2 gvresult ->
   sInsn (mkCfg S TD Ps gl fs)
     (mkState (mkEC F B ((insn_select id v0 t v1 v2)::cs) tmn lc als) (ECS) Mem)
     (mkState (mkEC F B cs tmn (updateAddAL _ lc id gvresult) als) (ECS) Mem)
